move different invariants to subdirectories

theories/simplang/simple_inv/simple_inv_refl.v
@@ -1,6 +1,7 @@
 From simuliris.simulation Require Import slsls lifting.
 From simuliris.simplang Require Import proofmode tactics.
-From simuliris.simplang Require Import parallel_subst heap_bij_races log_rel ctx.
+From simuliris.simplang Require Import parallel_subst log_rel ctx.
+From simuliris.simplang.simple_inv Require Import simple_inv.
 
 (** * Reflexivity theorem for the heap bijection value relation *)
 
@@ -11,20 +12,19 @@ This is basically our 'type system'. Indeed, "no types" really just means
 Definition expr_wf (e : expr) : Prop :=
   match e with
   | Val v => val_wf v
-  | Load o e => o ≠ Na2Ord
-  | Store o e1 e2 => o ≠ Na2Ord
   | CmpXchg e1 e2 e3 => False   (* currently not supported *)
   | FAA e1 e2 => False          (* currently not supported *)
   | _ => True
   end.
 
 Section refl.
-  Context `{nabijG Σ}.
+  Context `{heapbijG Σ}.
+  Notation log_rel := (log_rel val_rel (const True%I)) (only parsing).
 
-  Theorem expr_wf_sound : log_rel_exprs expr_wf val_rel (λ π, na_locs π ∅).
+  Theorem expr_wf_sound : log_rel_exprs expr_wf val_rel (const True%I).
   Proof.
     intros e_t e_s Hwf Hs. iIntros "IH".
-    destruct e_s, e_t => //=; simpl in Hs; simplify_eq.
+    destruct e_s, e_t => //; simpl in Hs; simplify_eq.
     all: try iDestruct "IH" as "[IH IH1]".
     all: try iDestruct "IH1" as "[IH1 IH2]".
     all: try iDestruct "IH2" as "[IH2 IH3]".
@@ -33,7 +33,7 @@ Section refl.
     - (* Let *) by iApply (log_rel_let with "IH IH1").
     - (* Call *)
       iApply (log_rel_call with "IH IH1").
-      by iIntros (???).
+      iIntros (???). by rewrite left_id.
     - (* UnOp *) by iApply (log_rel_unop with "IH").
     - (* BinOp *) by iApply (log_rel_binop with "IH IH1").
     - (* If *) by iApply (log_rel_if with "IH IH1 IH2").
@@ -43,13 +43,16 @@ Section refl.
     - (* Snd *) by iApply (log_rel_snd with "IH").
     - (* InjL *) by iApply (log_rel_injl with "IH").
     - (* InjR *) by iApply (log_rel_injr with "IH").
-    - (* Match *) destruct_and!; simplify_eq. by iApply (log_rel_match with "IH IH1 IH2").
+    - (* Match *) destruct_and!; simplify_eq.
+      by iApply (log_rel_match with "IH IH1 IH2").
     - (* Fork *)
       iApply (log_rel_fork with "IH").
-      iIntros (????) "Ht Hsim Hfork". by iApply (sim_bij_fork with "Ht Hsim").
+      iIntros (?????) "Hsim Hfork". iApply (sim_fork with "(Hsim [//])").
+      iIntros (?). iApply (sim_wand with "[Hfork]"). { by iApply "Hfork". }
+      iIntros (??) "[_ $]".
     - (* AllocN *)
       iApply (log_rel_allocN with "IH IH1").
-      iIntros (??????) "Ht Hv Hcont".
+      iIntros (???????) "Hv Hcont".
       target_alloc l_t as "Hl_t" "Ha_t"; first done.
       source_alloc l_s as "Hl_s" "Ha_s"; first done.
       iApply (sim_bij_insertN with "Ha_t Ha_s Hl_t Hl_s [Hv]"); [lia | by rewrite replicate_length.. | | ].
@@ -61,16 +64,13 @@ Section refl.
       by iApply "Hcont".
     - (* FreeN *)
       iApply (log_rel_freeN with "IH IH1").
-      iIntros (??????) "Ht Hv Hcont". by iApply (sim_bij_free with "Hv Ht").
+      iIntros (???????) "Hv Hcont". sim_free. by iApply "Hcont".
     - (* Load *)
       iApply (log_rel_load with "IH").
-      iIntros (????) "Ht Hv Hcont". iApply (sim_bij_load with "Hv Ht"); [done..|].
-      iIntros (??) "H ?". by iApply ("Hcont" with "[$]").
+      iIntros (?????) "Hv Hcont". iApply (sim_bij_load with "Hv"). iIntros (??). by iApply "Hcont".
     - (* Store *)
       iApply (log_rel_store with "IH IH1").
-      iIntros (??????) "Ht Hl Hv Hcont".
-      destruct o => //.
-      + by iApply (sim_bij_store_sc with "Hl Ht Hv").
-      + by iApply (sim_bij_store_na with "Hl Ht Hv").
+      iIntros (???????) "Hl Hv Hcont". iApply (sim_bij_store with "Hl Hv"). by iApply "Hcont".
   Qed.
+
 End refl.
