theories/simplang/na_inv/examples/data_races.v
@@ -1,8 +1,9 @@
-From simuliris.simplang Require Import lang notation tactics class_instances proofmode heap_bij_races.
+From simuliris.simplang Require Import lang notation tactics class_instances proofmode.
 From iris Require Import bi.bi.
 Import bi.
 From iris.proofmode Require Import tactics.
 From simuliris.simulation Require Import slsls lifting.
+From simuliris.simplang.na_inv Require Export na_inv.
 
 (** * Examples for exploiting UB of data-races. *)
 
