theories/simplang/na_inv/na_inv.v
@@ -5,7 +5,8 @@ From simuliris.base_logic Require Export gen_sim_heap gen_sim_prog.
 From simuliris.simulation Require Import slsls lifting.
 From iris.algebra.lib Require Import gset_bij.
 From iris.base_logic.lib Require Import gset_bij.
-From simuliris.simplang Require Export class_instances primitive_laws na_locs heapbij.
+From simuliris.simplang Require Export class_instances primitive_laws heapbij.
+From simuliris.simplang.na_inv Require Export na_locs.
 
 From iris.prelude Require Import options.
 
